% Created 2020-12-20 Sun 23:25
% Intended LaTeX compiler: pdflatex
\documentclass[11pt]{article}
\usepackage[utf8]{inputenc}
\usepackage[T1]{fontenc}
\usepackage{graphicx}
\usepackage{grffile}
\usepackage{longtable}
\usepackage{wrapfig}
\usepackage{rotating}
\usepackage[normalem]{ulem}
\usepackage{amsmath}
\usepackage{textcomp}
\usepackage{amssymb}
\usepackage{capt-of}
\usepackage{hyperref}
\author{Christian Påbøl}
\date{\today}
\title{Weekly 4}
\hypersetup{
 pdfauthor={Christian Påbøl},
 pdftitle={Weekly 4},
 pdfkeywords={},
 pdfsubject={},
 pdfcreator={Emacs 27.1 (Org mode 9.3)}, 
 pdflang={English}}
\begin{document}

\maketitle
\tableofcontents

\section{{\bfseries\sffamily TODO} Task 1}
\label{sec:orgbd126b1}
\section{Task 2}
\label{sec:orgadc6425}
In lecture 8, on slide 41 we are given the mathematical formulas for
calculating the adjoint values of a \texttt{scan (*)} statement. I wrote this
up in futhark. I also inlined the partial differentials. Setting the
last in lines 3 and 4 is done using an if in a map. Had this been written
with a less strict type system in mind, i might have either used list
concatenation or a "shift" operation, however futhark doesn't like manual
list operations \emph{nor} operations on only one index. Therefore, it is a
map
\begin{verbatim}
1  let scanAdjoint [n] (as: [n]real) (ys_bar_0: [n]real) : [n]real =
2    let ys = scan (*) 1.0 as
3    let is = iota n
4    let cs = map (\i -> if i == n-1 then 1 else as[i+1]) is
5    let ds = map (\i -> if i == n-1 then 0 else ys_bar_0[i]) is
6    let ys_bar = scan lin_o (0, 1) (zip (reverse ds) (reverse cs))
7      |> map (\ (d, c) -> d + (c * ys_bar_0[n-1]) )
8      |> reverse
9    in map (\i -> if i == 0 then ys_bar[0] else (ys[i-1]*ys_bar[i])) is
\end{verbatim}
It does validate.

\section{Task 3}
\label{sec:org9f0d3cf}

We are given the following code
\begin{verbatim}
forall i = 0 .. N-1 do
  forall j = 0 .. N-1 do
    let ps = map (*) A[i,:] B[:,j]
    let c = reduce (+) 0.0 ps

    let r_bar = C[i,j]
    let ps_bar = replicate N 0.0 -- init

    let ps_bar = map (+r) ps_bar

    forall k = 0 .. N-1 do
      let A_bar[i,k] += B[k,j] * ps_bar[k]
      let B_bar[k,j] += A[i,k] * ps_bar[k]
\end{verbatim}
I look at this and see that i am supposed to rewrite this as two nested
maps, which the compiler can optimize with tiling. I am also given a
rough map of what transformations to apply. Starting with DBE:  

\begin{itemize}
\item \texttt{c} is never used. Yeet that shizzle
\item \texttt{ps} is redundant also, get outta here
\end{itemize}
\begin{verbatim}
forall i = 0 .. N-1 do
  forall j = 0 .. N-1 do

    let r_bar = C[i,j]
    let ps_bar = replicate N 0.0

    let ps_bar = map (+r_bar) ps_bar

    forall k = 0 .. N-1 do
      let A_bar[i,k] += B[k,j] * ps_bar[k]
      let B_bar[k,j] += A[i,k] * ps_bar[k]
\end{verbatim}

We then simplify the definition of \texttt{ps\_bar} and inline \texttt{r}

\begin{verbatim}
forall i = 0 .. N-1 do
  forall j = 0 .. N-1 do
    let ps_bar = replicate N C[i,j]
    forall k = 0 .. N-1 do
      let A_bar[i,k] += B[k,j] * ps_bar[k]
      let B_bar[k,j] += A[i,k] * ps_bar[k]
\end{verbatim}

And then we see that ps\textsubscript{bar} can be eliminated completely
\begin{verbatim}
forall i = 0 .. N-1 do
  forall j = 0 .. N-1 do
    forall k = 0 .. N-1 do
      let A_bar[i,k] += B[k,j] * C[i,j]
      let B_bar[k,j] += A[i,k] * C[i,j]
\end{verbatim}

We perform some loop distribution and interchange
\begin{verbatim}
forall i = 0 .. N-1 do
  forall k = 0 .. N-1 do
    let acc = 0.0
    forall j = 0 .. N-1 do
      acc += B[k,j] * C[i,j] 
    A_bar[i,k] = acc

forall j = 0 .. N-1 do
  forall k = 0 .. N-1 do
    let acc = 0.0
    forall i = 0 .. N-1 do
      acc += A_T[k,i] * C[i,j]
    let B_bar[k,j] = acc
\end{verbatim}

And finally we are ready to rewrite this as a series of maps
Which can be optimised  

I start with the first A\textsubscript{bar} calculation, going through the following
steps, starting with the innermost loop.\footnote{While rules were on the
slides, i didn't understand till i went through these steps so i wanted
to include them}
\begin{verbatim}
forall i = 0 .. N-1 do
  forall k = 0 .. N-1 do
    let acc = 0.0
    forall j = 0 .. N-1 do
      acc += B[k,j] * C[i,j] 
    A_bar[i,k] = acc

forall i = 0 .. N-1 do
  forall k = 0 .. N-1 do
    map2 (*) B[k] C[i] |> reduce (+) 0.0

forall i = 0 .. N-1 do
  map (B_row -> 
    map2 (*) B_row C[i] |> reduce (+) 0.0
  ) 
map (C_row ->
  map (B_row -> 
    map2 (*) B_row C_row |> reduce (+) 0.0
  ) B
) C
\end{verbatim}

I then perform a similar transformation for the values of \texttt{B\_bar}, while
remembering to transpose the right variables. I interchange the two
outer loops, since the indexing of B and A are reversed.
\begin{verbatim}
let B_bar =
map (\A_T_row ->
  map (\C_t_r ->
    map2 (*) A_T[k] C_t_r
    ) (transpose C)
  ) (transpose A)
\end{verbatim}

The final fully optimized code is:
\begin{verbatim}
let A_bar =
map (C_row ->
  map (B_row -> 
    map2 (*) B_row C_row |> reduce (+) 0.0
  ) B
) C
let B_bar =
map (\A_T_row ->
  map (\C_t_r ->
    map2 (*) A_T[k] C_t_r
    ) (transpose C)
  ) (transpose A)
\end{verbatim}
\end{document}
